Restructured and proved all other lemmas.

HBRaceDetector.v
@@ -5,49 +5,40 @@ Require Import conc_model.
 Require Import SCFacts.
 Require Import Lang.
 Require Import FunctionalExtensionality.
+Require Import ExecFacts.
 Set Implicit Arguments.
 
 Definition move src tgt tmp := [Load tmp src; Store tgt (V tmp)].
-
-Lemma upd_same : forall G t a v,
-  (upd_env G t a v) t a = v.
-Proof.
-  unfold upd_env, upd; clarify.
-Qed.
-
-Lemma upd_overwrite : forall G t a v1 v2,
-  upd_env (upd_env G t a v1) t a v2 = upd_env G t a v2.
-Proof.
-  intros; extensionality t'; extensionality v'.
-  unfold upd_env, upd; clarify.
-Qed.
 
 Definition events_move (src tgt:var) (t:tid): list operation :=
   [rd t src; wr t tgt].
 
 Definition mops_move (src tgt: ptr) (t:tid) (v:nat): list conc_op := [Read t src v; Write t tgt v].
 
-Lemma move_spec : forall src tgt i j tmp P P1 P2 G t rest v
+Lemma move_spec_t : forall src tgt i j tmp P P1 P2 G t rest v
+  (Hmove : P = P1 ++ (t, move (src, i) (tgt, j) tmp ++ rest) :: P2),
+  exec_star_t t (Some P) G
+            (events_move src tgt t) (mops_move (src, i) (tgt, j) t v)
+    (Some (P1 ++ (t, rest) :: P2)) (upd_env G t tmp v).
+Proof.
+  clarify.
+  eapply exec_step_t'.
+  - apply exec_load; eauto.
+  - eapply exec_step_t'; auto.
+    + apply exec_store; eauto.
+    + apply exec_refl_t.
+  - auto.
+  - simpl.
+    rewrite upd_same; auto.
+Qed.
+
+Corollary move_spec : forall src tgt i j tmp P P1 P2 G t rest v
   (Hmove : P = P1 ++ (t, move (src, i) (tgt, j) tmp ++ rest) :: P2),
   exec_star (Some P) G
             (events_move src tgt t) (mops_move (src, i) (tgt, j) t v)
     (Some (P1 ++ (t, rest) :: P2)) (upd_env G t tmp v).
 Proof.
-  intros. 
-  eapply exec_step'.
-  - apply exec_load.
-    unfold move in Hmove.  eauto.
-  - simpl.
-    eapply exec_step'.
-    + apply exec_store.
-      eauto.
-    + apply exec_refl.
-    + auto.
-    + auto.
-  - auto.
-  - simpl.
-    rewrite upd_same.
-    auto.
+  intros; eapply exec_t_exec, move_spec_t; auto.
 Qed.
 
 Fixpoint set_vc (src : var (* loc of source VC *)) (tgt : var (* loc of target VC *))
@@ -76,36 +67,22 @@ Proof.
   destruct vs; clarify.
 Qed.
 
-Lemma set_vc_spec_0 : forall src tgt tmp P G P1 P2 t rest 
-(Hset_vc0: P=P1++(t, set_vc src tgt 0 tmp ++ rest)::P2),
-exec_star (Some P) G [] [] (Some (P1++(t,rest)::P2)) G.
-Proof.
-  intros.
-  unfold set_vc in Hset_vc0.
-  rewrite Hset_vc0.
-  simpl.
-  eapply exec_refl.
-Qed.
-
 Lemma events_set_vc_step: forall src tgt n t,
   events_set_vc src tgt (S n) t = (events_move src tgt t)++events_set_vc src tgt n t.
 Proof.
-  intros.
-  eauto.
+  auto.
 Qed.
 
 Lemma mops_set_vc_step: forall src tgt n t v vss,
   mops_set_vc src tgt (S n) t (v::vss)= (mops_move (src,n) (tgt,n) t v)++mops_set_vc src tgt n t vss.
 Proof.
-  intros.
-  eauto.
+  auto.
 Qed.
 
 Lemma set_vc_step: forall  src tgt n tmp,
   set_vc src tgt (S n) tmp =(move (src,n) (tgt,n) tmp)++set_vc src tgt n tmp.
 Proof.
-  intros.
-  eauto.
+  auto.
 Qed.
 
 Lemma nonempty_list: forall (ls : list nat) n, 
@@ -114,74 +91,42 @@ Proof.
   destruct ls; clarify; eauto.
 Qed.
 
-Lemma set_vc_spec_step : forall src tgt n tmp P G P1 P2 t rest v 
-(Hset_vc: P=P1++(t, set_vc src tgt (S n) tmp++ rest)::P2),
- exec_star (Some P) G
-          (events_move src tgt t) (mops_move (src,n) (tgt,n) t v) (Some (P1++(t, set_vc src tgt n tmp++rest)::P2)) (upd_env G t tmp v).
+Opaque last.
+
+Lemma set_vc_spec_t : forall n src tgt tmp P G P1 P2 t rest vss 
+(Hset_vc: P=P1++(t, set_vc src tgt n tmp++ rest)::P2) (Hvs: length vss=n),
+ exec_star_t t (Some P) G (events_set_vc src tgt n t)
+             (mops_set_vc src tgt n t vss)
+             (Some (P1++(t,rest)::P2)) (upd_env G t tmp (last vss (G t tmp))).
 Proof.
-  intros.
-  rewrite Hset_vc.
-  rewrite set_vc_step.
-  apply move_spec.
-  auto.
+  induction n; destruct vss; clarify.
+  - rewrite upd_triv; apply exec_refl_t.
+  - eapply exec_step_t'.
+    { apply exec_load; eauto. }
+    eapply exec_step_t'; auto.
+    { apply exec_store; eauto. }
+    instantiate (1 := mops_set_vc src tgt n t vss).
+    instantiate (1 := events_set_vc src tgt n t).
+    instantiate (1 := n0).
+    destruct (nil_dec vss); clarify.
+    + destruct n; clarify.
+      apply exec_refl_t.
+    + rewrite last_cons; auto.
+      exploit IHn; eauto.
+      instantiate (3 := upd_env G t tmp n0).
+      rewrite upd_overwrite, upd_same.
+      erewrite last_def; eauto.
+    + auto.
+    + simpl.
+      rewrite upd_same; auto.
 Qed.
 
-Lemma set_vc_spec_n : forall n src tgt tmp P G P1 P2 t rest v vss 
-(Hset_vc: P=P1++(t, set_vc src tgt (S n) tmp++ rest)::P2) (Hvs: length vss=n),
- exec_star (Some P) G
-          (events_set_vc src tgt (S n) t) (mops_set_vc src tgt (S n) t (vss++[v])) (Some (P1++(t,rest)::P2)) (upd_env G t tmp v).
-Proof.
-  
-  intros n.
-  induction n.
-
-  -intros.
-   apply empty_list in Hvs.
-   clarify.
-   apply move_spec.
-   eauto.  
-  -intros.
-   rewrite Hset_vc.
-   (*
-   eapply set_vc_spec_step in Hset_vc.
-   rewrite set_vc_step in Hset_vc.*)
-   apply nonempty_list in Hvs.
-   inversion Hvs.
-   inversion H.
-   inversion H0.
-   rewrite H1.
-   rewrite list_cons_plus_assoc.
-   rewrite events_set_vc_step,mops_set_vc_step, set_vc_step.
-   eapply exec_star_trans.
-   +rewrite <- set_vc_step.
-    apply set_vc_spec_step.
-    eauto.
-   +assert( Hupd: upd_env G t tmp v = upd_env (upd_env G t tmp x) t tmp v).  
-    rewrite upd_overwrite. auto.
-    rewrite Hupd.
-    apply IHn.
-    *auto.
-    *auto.
-Qed.
-
-Lemma upd_triv : forall G t a, upd_env G t a (G t a) = G.
-Proof.
-  intros; extensionality t'; extensionality a'; unfold upd_env, upd; clarify.
-Qed.
- 
 Corollary set_vc_spec : forall n src tgt tmp P G P1 P2 t rest vss 
 (Hset_vc: P=P1++(t, set_vc src tgt n tmp++ rest)::P2) (Hvs: length vss=n),
  exec_star (Some P) G (events_set_vc src tgt n t) (mops_set_vc src tgt n t vss)
   (Some (P1++(t,rest)::P2)) (upd_env G t tmp (last vss (G t tmp))).
 Proof.
-  destruct n; intros.
-  - destruct vss; clarify.
-    rewrite upd_triv; apply exec_refl.
-  - intros.
-    assert (vss <> []) as Hnnil by (destruct vss; clarify).
-    rewrite (app_removelast_last (G t tmp) Hnnil) in *.
-    rewrite last_snoc; apply set_vc_spec_n; auto.
-    rewrite app_length in *; clarify; omega.
+  intros; eapply exec_t_exec, set_vc_spec_t; auto.
 Qed.
  
 Definition inc_vc t tgt tmp := [
@@ -192,71 +137,38 @@ Definition inc_vc t tgt tmp := [
 
 Definition events_inc_vc (tgt:var) (t:tid): list operation:=
   [rd t tgt; wr t tgt]. 
-Definition mops_inc_vc (tgt:var) (v:nat) (t:tid): list conc_op:=
-  [Read t (tgt,t) v; Write t (tgt,t) (v+1) ].
 Definition mops_inc_vc' (tgt: var) (v: nat) (t t' :tid): list conc_op:=
   [Read t (tgt,t') v; Write t (tgt, t') (v+1)].
-Lemma inc_vc_spec' : forall  tgt tmp P G P1 P2 rest v t t'
+Notation mops_inc_vc tgt v t := (mops_inc_vc' tgt v t t).
+
+Lemma inc_vc_spec_t : forall  tgt tmp P G P1 P2 rest v t t'
+  (Hinc_vc: P=P1++((t,inc_vc t' tgt tmp++rest)::P2)),
+  exec_star_t t (Some P) G 
+            (events_inc_vc tgt t) (mops_inc_vc' tgt v t t') 
+            (Some (P1++(t,rest)::P2)) (upd_env G t tmp (v+1)). 
+Proof.
+  clarify.
+  eapply exec_step_t'.
+  { apply exec_load; eauto. }
+  eapply exec_step_t'; auto.
+  { apply exec_assign; eauto. }
+  rewrite upd_overwrite; simpl.
+  rewrite upd_same.
+  eapply exec_step_t'; auto.
+  { apply exec_store; eauto. }
+  apply exec_refl_t.
+  - auto. 
+  - simpl.
+    rewrite upd_same; auto.
+Qed.
+
+Corollary inc_vc_spec : forall  tgt tmp P G P1 P2 rest v t t'
   (Hinc_vc: P=P1++((t,inc_vc t' tgt tmp++rest)::P2)),
   exec_star (Some P) G 
             (events_inc_vc tgt t) (mops_inc_vc' tgt v t t') 
             (Some (P1++(t,rest)::P2)) (upd_env G t tmp (v+1)). 
 Proof.
-  intros.
-  eapply exec_step'.
-  -apply exec_load.
-   unfold inc_vc in Hinc_vc; eauto.
-  -simpl.
-   eapply exec_step'.
-   +apply exec_assign; eauto.
-   +simpl.
-    
-    eapply exec_step'.
-    *apply exec_store; eauto.
-    *rewrite upd_same.
-     rewrite upd_overwrite.
-     apply exec_refl.
-    *auto.
-    *auto.
-   +auto.
-   +auto.
-  -auto. 
-  -simpl.
-   unfold mops_inc_vc'.
-   repeat rewrite upd_same.
-   auto.
-Qed.
-
-
-Lemma inc_vc_spec : forall  tgt tmp P G P1 P2 rest v t 
-  (Hinc_vc: P=P1++((t,inc_vc t tgt tmp++rest)::P2)),
-  exec_star (Some P) G 
-            (events_inc_vc tgt t) (mops_inc_vc tgt v t) 
-            (Some (P1++(t,rest)::P2)) (upd_env G t tmp (v+1)). 
-Proof.
-  intros.
-  eapply exec_step'.
-  -apply exec_load.
-   unfold inc_vc in Hinc_vc; eauto.
-  -simpl.
-   eapply exec_step'.
-   +apply exec_assign; eauto.
-   +simpl.
-    
-    eapply exec_step'.
-    *apply exec_store; eauto.
-    *rewrite upd_same.
-     rewrite upd_overwrite.
-     apply exec_refl.
-    *auto.
-    *auto.
-   +auto.
-   +auto.
-  -auto.
-  -simpl.
-   unfold mops_inc_vc.
-   repeat rewrite upd_same.
-   auto.
+  intros; eapply exec_t_exec, inc_vc_spec_t; auto.
 Qed.
 
 Definition max src tgt tmp1 tmp2 :=
@@ -279,55 +191,36 @@ Definition mops_max (src tgt: ptr) (v1 v2 : nat) (t:tid): list conc_op:=
   Read t src v1;
   Read t tgt v2;
   Write t tgt (Peano.max v1 v2)
-  (*;Write t tgt (nat.max v1 v2)*)
 ].
-Lemma upd_diff : forall G t a1 a2 v1 v2
- (Ha: a1<>a2),
- (upd_env (upd_env G t a1 v1) t a2 v2) t a1 = v1. 
-Proof.
-  intros; unfold upd_env, upd; clarify.
-Qed.
 
-Lemma upd_assoc: forall G t a1 a2 v1 v2
- (Ha: a1<>a2),
- upd_env (upd_env G t a1 v1) t a2 v2 = upd_env (upd_env G t a2 v2) t a1 v1.
-Proof.
-  intros; extensionality t'; extensionality v'.
-  unfold upd_env, upd; clarify.
-Qed.
-
-Lemma max_spec : forall P P1 P2 rest G src tgt i j tmp1 tmp2 v1 v2 t
+Lemma max_spec_t : forall P P1 P2 rest G src tgt i j tmp1 tmp2 v1 v2 t
  (Hmax_spec: P= P1++((t, max (src, i) (tgt, j) tmp1 tmp2++rest)::P2)) (Hdist: tmp1<> tmp2),
-exec_star (Some P) G (events_max src tgt t) (mops_max (src, i) (tgt, j) v1 v2 t) (Some (P1++(t,rest)::P2)) (upd_env (upd_env G t tmp1 v1) t tmp2 (Peano.max v1 v2)).  
+exec_star_t t (Some P) G (events_max src tgt t) (mops_max (src, i) (tgt, j) v1 v2 t) (Some (P1++(t,rest)::P2)) (upd_env (upd_env G t tmp1 v1) t tmp2 (Peano.max v1 v2)).  
 Proof.
-  intros.
-  rewrite Hmax_spec.
-  eapply exec_step'.
-  -apply exec_load.
-   unfold max. clarify.
-  -eapply exec_step'.
-   +apply exec_load. clarify.
-   +eapply exec_step'.
-    *apply exec_assign. clarify.
-    *clarify.
-     
-     eapply exec_step'.
-      apply exec_store. eauto.
-      rewrite upd_overwrite. 
-      repeat rewrite upd_same.
-      rewrite upd_diff. apply exec_refl.
-      eauto.
-      eauto.
-      eauto.
-    *eauto.
-    *eauto.
-   +eauto.
-   +eauto.
-  -eauto.
-  -eauto.
-   unfold mops_max. clarify. repeat rewrite upd_same. rewrite upd_diff; eauto.
+  clarify.
+  eapply exec_step_t'.
+  { apply exec_load; eauto. }
+  eapply exec_step_t'; auto.
+  { apply exec_load; eauto. }
+  eapply exec_step_t'; auto.
+  { apply exec_assign; eauto. }
+  rewrite upd_overwrite; simpl.
+  rewrite upd_old, upd_same, upd_same; auto.
+  eapply exec_step_t'; auto.
+  { apply exec_store; auto. }
+  apply exec_refl_t.
+  - auto.
+  - simpl.
+    rewrite upd_same; auto.
 Qed.
  
+Corollary max_spec : forall P P1 P2 rest G src tgt i j tmp1 tmp2 v1 v2 t
+ (Hmax_spec: P= P1++((t, max (src, i) (tgt, j) tmp1 tmp2++rest)::P2)) (Hdist: tmp1<> tmp2),
+exec_star (Some P) G (events_max src tgt t) (mops_max (src, i) (tgt, j) v1 v2 t) (Some (P1++(t,rest)::P2)) (upd_env (upd_env G t tmp1 v1) t tmp2 (Peano.max v1 v2)).
+Proof.
+  intros; eapply exec_t_exec, max_spec_t; auto.
+Qed.
+
 Fixpoint max_vc src tgt z tmp1 tmp2 :=
 match z with
 | 0 => []
@@ -346,110 +239,61 @@ match (z,vs1,vs2) with
 |(S n,v1::vss1,v2::vss2) => mops_max (src,n) (tgt,n) v1 v2 t ++ mops_max_vc src tgt vss1 vss2 t n
 | _ => []
 end. 
-Lemma max_vc_spec_0 : forall src tgt tmp1 tmp2 P G P1 P2 t rest
-(Hmax_vc0 : P=P1++(t, max_vc src tgt 0 tmp1 tmp2 ++ rest)::P2),
- exec_star (Some P) G 
-           [] [] (Some (P1++(t,rest)::P2)) G.
-Proof.
-  intros.
-  unfold max_vc in Hmax_vc0.
-  rewrite Hmax_vc0.
-  eapply exec_refl.
-Qed.
-
 
 Lemma events_max_vc_step: forall src tgt t n,
   events_max_vc src tgt t (S n) = events_max src tgt t ++ events_max_vc src tgt t n.
 Proof.
-  intros.
-  eauto.
+  auto.
 Qed.
 
 Lemma mops_max_vc_step: forall src tgt n v1 v2 vss1 vss2 t,
   mops_max_vc src tgt (v1::vss1) (v2::vss2) t (S n) =
   mops_max (src,n) (tgt,n) v1 v2 t ++ mops_max_vc src tgt vss1 vss2 t n.
 Proof.
-  intros.
-  eauto.
+  auto.
 Qed.
 
 Lemma max_vc_step: forall  src tgt n tmp1 tmp2,
   max_vc src tgt (S n) tmp1 tmp2 = max (src,n) (tgt,n) tmp1 tmp2++ max_vc src tgt  n tmp1 tmp2.
 Proof.
-  intros.
-  eauto.
+  auto.
 Qed.
 
-Lemma max_vc_spec_step : forall n src tgt tmp1 tmp2 P G P1 P2 t rest v1 v2
-
-(Hmax_vc: P=P1++(t, max_vc src tgt (S n) tmp1 tmp2 ++ rest)::P2) (Htmp: tmp1 <> tmp2),
- exec_star (Some P) G
-          (events_max src tgt t) (mops_max (src,n) (tgt,n) v1 v2 t) (Some (P1++(t, max_vc src tgt n tmp1 tmp2 ++ rest)::P2)) (upd_env (upd_env G t tmp1 v1) t tmp2 (Peano.max v1 v2)).
+Lemma max_vc_spec_t : forall n src tgt tmp1 tmp2 P G P1 P2 t rest vss1
+  vss2 (Hmax_vc: P=P1++(t, max_vc src tgt n tmp1 tmp2 ++ rest)::P2)
+  (Htmp: tmp1 <> tmp2) (Hvs1: length vss1=n) (Hvs2: length vss2=n),
+  exec_star_t t (Some P) G (events_max_vc src tgt t n)
+    (mops_max_vc src tgt vss1 vss2 t n) (Some (P1++(t,rest)::P2))
+    (upd_env (upd_env G t tmp1 (last vss1 (G t tmp1))) t tmp2
+      (last (map (fun x => Peano.max (fst x) (snd x)) (combine vss1 vss2))
+      (G t tmp2))).
 Proof.
-  intros.
-  rewrite Hmax_vc.
-  rewrite max_vc_step.
-  apply max_spec; eauto.
-Qed.
-  
-Lemma max_vc_spec_n : forall n src tgt tmp1 tmp2 P G P1 P2 t rest v1 v2 vss1 vss2
-
-(Hmax_vc: P=P1++(t, max_vc src tgt (S n) tmp1 tmp2 ++ rest)::P2) (Htmp: tmp1 <> tmp2) (Hvs1: length vss1=n) (Hvs2: length vss2=n),
- exec_star (Some P) G
-          (events_max_vc src tgt t (S n)) (mops_max_vc src tgt (vss1++[v1]) (vss2++[v2]) t (S n)) (Some (P1++(t,rest)::P2)) (upd_env (upd_env G t tmp1 v1) t tmp2 (Peano.max v1 v2)).
-Proof.
-  intro n.
-  induction n.
-  -intros.
-   apply empty_list in Hvs1.
-   apply empty_list in Hvs2.
-   rewrite Hvs1, Hvs2. simpl.
-   apply max_spec; eauto.
-
-  -intros.
-   rewrite Hmax_vc.
-   apply nonempty_list in Hvs1.
-   apply nonempty_list in Hvs2.
-   inversion Hvs1.
-   inversion Hvs2.
-   inversion H.
-   inversion H0.
-   inversion H1.
-   inversion H2.
-   rewrite H3, H5.
-   repeat rewrite list_cons_plus_assoc.
-   rewrite events_max_vc_step, mops_max_vc_step, max_vc_step.
-   eapply exec_star_trans.
-   +apply max_vc_spec_step; eauto.
-    rewrite <- max_vc_step. eauto.
-   +assert(Hupd: (upd_env (upd_env G t tmp1 v1) t tmp2 (Peano.max v1 v2)) = upd_env (upd_env (upd_env (upd_env G t tmp1 x) t tmp2 (Peano.max x x0)) t tmp1 v1) t tmp2 (Peano.max v1 v2)).
-    symmetry.
-    rewrite upd_assoc.
-    rewrite upd_overwrite.
-    rewrite upd_assoc.
-    rewrite upd_overwrite. eauto.
-    auto. apply Htmp.
-   rewrite Hupd. 
-   apply IHn; eauto.
+  induction n; destruct vss1, vss2; intros; subst; try solve [clarify].
+  - do 2 rewrite upd_triv; apply exec_refl_t.
+  - rewrite max_vc_step, events_max_vc_step, mops_max_vc_step.
+    eapply exec_star_t_trans; [apply max_spec_t; eauto; reflexivity|].
+    exploit IHn.
+    { eauto. }
+    { eauto. }
+    { instantiate (1 := vss1); clarify. }
+    { instantiate (1 := vss2); clarify. }
+    simpl; do 2 rewrite last_cons'.
+    instantiate (2 := upd_env (upd_env G t tmp1 n0) t tmp2 (Peano.max n0 n1)).
+    rewrite upd_three, upd_three; auto.
+    rewrite upd_same, upd_assoc, upd_same; eauto.
 Qed.
 
 Corollary max_vc_spec : forall n src tgt tmp1 tmp2 P G P1 P2 t rest vss1
   vss2 (Hmax_vc: P=P1++(t, max_vc src tgt n tmp1 tmp2 ++ rest)::P2)
   (Htmp: tmp1 <> tmp2) (Hvs1: length vss1=n) (Hvs2: length vss2=n),
-  exists v1 v2, exec_star (Some P) G (events_max_vc src tgt t n)
+  exec_star (Some P) G (events_max_vc src tgt t n)
     (mops_max_vc src tgt vss1 vss2 t n) (Some (P1++(t,rest)::P2))
-    (upd_env (upd_env G t tmp1 v1) t tmp2 v2).
+    (upd_env (upd_env G t tmp1 (last vss1 (G t tmp1))) t tmp2
+      (last (map (fun x => Peano.max (fst x) (snd x)) (combine vss1 vss2))
+      (G t tmp2))).
 Proof.
-  destruct n; intros.
-  - destruct vss1, vss2; clarify.
-    do 2 eexists; repeat rewrite upd_triv; apply exec_refl.
-  - assert (vss1 <> []) as Hnnil1 by (destruct vss1; clarify).
-    assert (vss2 <> []) as Hnnil2 by (destruct vss2; clarify).
-    rewrite (app_removelast_last 0 Hnnil1) in *.
-    rewrite (app_removelast_last 0 Hnnil2) in *.
-    rewrite app_length in Hvs1, Hvs2.
-    do 2 eexists; apply max_vc_spec_n; clarify; omega.
-Qed.        
+  intros; eapply exec_t_exec, max_vc_spec_t; auto.
+Qed.
 
 Definition assert_le (a b : ptr) (tmp1 tmp2:local): prog :=
 [
@@ -470,56 +314,61 @@ Definition mops_assert_le (a b : ptr) (v1 v2: nat) (t: tid): list conc_op :=
   Read t b v2
 ].
 
-Lemma assert_le_fail_spec: forall P P1 P2 rest G a b i j tmp1 tmp2 t v1 v2
+Lemma assert_le_fail_spec_t : forall P P1 P2 rest G a b i j tmp1 tmp2 t v1 v2
+ (Hassert_le_spec: P=P1++(t,assert_le (a, i) (b, j) tmp1 tmp2++rest)::P2) (Htmp: tmp1<>tmp2) (Hv1v2: ~ v1 <= v2),
+ exec_star_t t (Some P) G (events_assert_le a b t) (mops_assert_le (a, i) (b, j) v1 v2 t)
+            None (upd_env (upd_env G t tmp1 v1) t tmp2 v2).
+Proof.
+  clarify.
+  eapply exec_step_t'.
+  { apply exec_load; auto. }
+  eapply exec_step_t'; auto.
+  { apply exec_load; auto. }
+  eapply exec_step_t'; auto.
+  { eapply exec_assert_fail; eauto.
+    simpl.
+    rewrite upd_old, upd_same, upd_same; eauto. }
+  apply exec_refl_t.
+  - auto.
+  - auto.
+Qed.
+
+Corollary assert_le_fail_spec: forall P P1 P2 rest G a b i j tmp1 tmp2 t v1 v2
  (Hassert_le_spec: P=P1++(t,assert_le (a, i) (b, j) tmp1 tmp2++rest)::P2) (Htmp: tmp1<>tmp2) (Hv1v2: ~ v1 <= v2),
  exec_star (Some P) G (events_assert_le a b t) (mops_assert_le (a, i) (b, j) v1 v2 t)
             None (upd_env (upd_env G t tmp1 v1) t tmp2 v2).
 Proof.
-  intros.
-  rewrite Hassert_le_spec.
-  eapply exec_step'.
-  -apply exec_load.
-   unfold assert_le.
-   clarify.
-  -eapply exec_step'.
-   +apply exec_load.
-    clarify.
-    +eapply exec_step'.
-     eapply exec_assert_fail. eauto.
-     unfold eval. rewrite upd_same. rewrite upd_assoc. rewrite upd_same. 
-     apply Hv1v2. apply Htmp. 
-     apply exec_refl.
-     eauto.
-     eauto.
-    +eauto.
-    +eauto.
-   -eauto.
-   -eauto.
+  intros; eapply exec_t_exec, assert_le_fail_spec_t; eauto.
 Qed.
 
+Lemma assert_le_pass_spec_t : forall P P1 P2 rest G a b i j tmp1 tmp2 t v1 v2
+ (Hassert_le_spec: P=P1++(t,assert_le (a, i) (b, j) tmp1 tmp2++rest)::P2) (Htmp: tmp1<>tmp2) (Hv1v2: v1 <= v2),
+ exec_star_t t (Some P) G (events_assert_le a b t) (mops_assert_le (a, i) (b, j) v1 v2 t)
+            (Some (P1++(t,rest)::P2)) (upd_env (upd_env G t tmp1 v1) t tmp2 v2).
+Proof.
+  clarify.
+  eapply exec_step_t'.
+  { apply exec_load; auto. }
+  eapply exec_step_t'; auto.
+  { apply exec_load; auto. }
+  eapply exec_step_t'; auto.
+  { eapply exec_assert_pass; eauto.
+    simpl.
+    rewrite upd_old, upd_same, upd_same; eauto. }
+  apply exec_refl_t.
+  - auto.
+  - auto.
+Qed.
+    
 Lemma assert_le_pass_spec: forall P P1 P2 rest G a b i j tmp1 tmp2 t v1 v2
  (Hassert_le_spec: P=P1++(t,assert_le (a, i) (b, j) tmp1 tmp2++rest)::P2) (Htmp: tmp1<>tmp2) (Hv1v2: v1 <= v2),
  exec_star (Some P) G (events_assert_le a b t) (mops_assert_le (a, i) (b, j) v1 v2 t)
             (Some (P1++(t,rest)::P2)) (upd_env (upd_env G t tmp1 v1) t tmp2 v2).
 Proof.
-  intros.
-  rewrite Hassert_le_spec.
-  eapply exec_step';eauto.
-  -apply exec_load.
-   unfold assert_le.
-   clarify.
-  -eapply exec_step';eauto.
-   +apply exec_load.
-    clarify.
-   +eapply exec_step';eauto.
-    *eapply exec_assert_pass; eauto.
-     unfold eval. rewrite upd_same. rewrite upd_assoc; eauto. rewrite upd_same.
-     apply Hv1v2.
-    *apply exec_refl.
-  -eauto.
-  -eauto.
+  intros; eapply exec_t_exec, assert_le_pass_spec_t; eauto.
 Qed.
-    
+  
+
 Fixpoint hb_check C1 C2 z tmp1 tmp2 :=
 match z with
 | 0 => []
@@ -529,8 +378,7 @@ end.
 Lemma hb_check_step: forall C1 C2 n tmp1 tmp2,
  hb_check C1 C2 (S n) tmp1 tmp2 = (assert_le (C1,n) (C2,n) tmp1 tmp2)++ hb_check C1 C2 n tmp1 tmp2.
 Proof.
-  intros.
-  eauto.
+  auto.
 Qed.
 
 Fixpoint events_hb_check (C1 C2: var) (vs1 vs2: list nat) (t:tid) : list operation :=
@@ -545,9 +393,8 @@ Lemma events_hb_check_step : forall C1 C2 v1 v2 vs1 vs2 t,
  events_assert_le C1 C2 t ++ 
  if leb v1 v2 then events_hb_check C1 C2 vs1 vs2 t else [].
 Proof.
-  intros. auto.
+  auto.
 Qed.
-
 
 
 Fixpoint mops_hb_check (C1 C2: var) (vs1 vs2: list nat) (z:nat) (t:tid) : list conc_op :=
@@ -563,46 +410,9 @@ Lemma mops_hb_check_step : forall C1 C2 v1 v2 vs1 vs2 n t,
  mops_assert_le (C1,n) (C2,n) v1 v2 t ++
  if leb v1 v2 then mops_hb_check C1 C2 vs1 vs2 n t else [].
 Proof.
-  intros. auto.
+  auto.
 Qed.
 
-Lemma hb_check_spec0: forall C1 C2 t tmp1 tmp2 P G P1 P2 rest
- (Hhb_check0: P=P1++(t,hb_check C1 C2 0 tmp1 tmp2++rest)::P2),
-  exec_star (Some P) G 
-            [] [] (Some (P1++(t,rest)::P2)) G.
-Proof.
-  intros.
-  unfold hb_check in Hhb_check0; eauto.
-  rewrite Hhb_check0.
-  apply exec_refl.
-Qed.
-
-Lemma hb_check_spec_step_fail: forall C1 C2 t tmp1 tmp2 P G P1 P2 rest n v1 v2
-  (Hhb_heck_step: P=P1++(t,hb_check C1 C2 (S n) tmp1 tmp2++rest)::P2) (Htmp: tmp1<> tmp2) (Hv1v2: ~ v1 <= v2),
-   exec_star (Some P) G (events_assert_le C1 C2 t)
-             (mops_assert_le (C1,n) (C2,n) v1 v2 t) 
-              None
-             (upd_env (upd_env G t tmp1 v1) t tmp2 v2).
-Proof.
-  intros.
-  rewrite Hhb_heck_step.
-  rewrite hb_check_step.
-  eapply assert_le_fail_spec; eauto;clarify.
-Qed.
- 
-Lemma hb_check_spec_step_pass: forall C1 C2 t tmp1 tmp2 P G P1 P2 rest n v1 v2
-  (Hhb_heck_step: P=P1++(t,hb_check C1 C2 (S n) tmp1 tmp2++rest)::P2) (Htmp: tmp1<> tmp2) (Hv1v2: v1 <= v2),
-   exec_star (Some P) G (events_assert_le C1 C2 t)
-             (mops_assert_le (C1,n) (C2,n) v1 v2 t) 
-             (Some (P1++(t,hb_check C1 C2 n tmp1 tmp2++rest)::P2))
-             (upd_env (upd_env G t tmp1 v1) t tmp2 v2).
-Proof.
-  intros.
-  rewrite Hhb_heck_step.
-  rewrite hb_check_step.
-  eapply assert_le_pass_spec; eauto; clarify.
-Qed.
-    
 Fixpoint first_gt l1 l2 :=
 match (l1,l2) with
 | (x1::xs1, x2::xs2) => if leb x1 x2 then first_gt xs1 xs2 else Some (x1,x2) 
@@ -612,48 +422,35 @@ end.
 Lemma first_gt_step: forall x1 x2 xs1 xs2,
 first_gt (x1::xs1) (x2::xs2) = if leb x1 x2 then first_gt xs1 xs2 else Some (x1,x2).
 Proof.
-  intros. eauto.
+  auto.
 Qed.
 
-Lemma hb_check_fail_spec_n: forall n C1 C2 t tmp1 tmp2 P G P1 P2 rest v1 v2 vs1 vs2
- (Hhb_check_spec: P= P1++(t,hb_check C1 C2 (S n) tmp1 tmp2++rest)::P2) 
- (Htmp: tmp1 <> tmp2) (Hvs1: length vs1 = S n) (Hvs2: length vs2 = S n) 
+Lemma hb_check_fail_spec_t : forall n C1 C2 t tmp1 tmp2 P G P1 P2 rest v1 v2
+  vs1 vs2 (Hhb_check_spec: P= P1++(t,hb_check C1 C2 n tmp1 tmp2++rest)::P2) 
+ (Htmp: tmp1 <> tmp2) (Hvs1: length vs1 = n) (Hvs2: length vs2 = n) 
  (Hfirst_gt: first_gt vs1 vs2 = Some (v1,v2)),
- exec_star (Some P) G (events_hb_check C1 C2 vs1 vs2 t)
-           (mops_hb_check C1 C2 vs1 vs2 (S n) t) 
-           None (upd_env (upd_env G t tmp1 v1) t tmp2 v2). 
+ exec_star_t t (Some P) G (events_hb_check C1 C2 vs1 vs2 t)
+   (mops_hb_check C1 C2 vs1 vs2 n t)
+   None (upd_env (upd_env G t tmp1 v1) t tmp2 v2).
 Proof.
-  intro n.
-  induction n;intros;
-  apply nonempty_list in Hvs1;apply nonempty_list in Hvs2;
-  inversion Hvs1; inversion Hvs2; inversion H; inversion H0;
-  inversion H1; inversion H2.
-  -apply empty_list in H4. apply empty_list in H6. clarify.
-   eapply assert_le_fail_spec;eauto.
-   +clarify.
-   +rewrite <- leb_le; intro; clarify.
-  - rewrite H3, H5, first_gt_step in Hfirst_gt. 
-    destruct (leb x x0) eqn:Hxx0; eauto.
-    +rewrite H3,H5. 
-     rewrite events_hb_check_step, mops_hb_check_step.
-     rewrite Hhb_check_spec, Hxx0,  hb_check_step.
-     eapply exec_star_trans.
-     *apply assert_le_pass_spec; clarify.
-      rewrite leb_le in *; auto.
-     *clarify.
-      assert(Hupd: (upd_env (upd_env G t tmp1 v1) t tmp2 v2)= upd_env (upd_env (upd_env (upd_env G t tmp1 x) t tmp2 x0) t tmp1 v1) t tmp2 v2).
-       symmetry. rewrite upd_assoc. rewrite upd_overwrite.
-       rewrite upd_assoc. rewrite upd_overwrite. eauto.
-       clarify. eauto.
-      rewrite Hupd.
-      eapply IHn; eauto.
-     +rewrite H3,H5.
-      rewrite events_hb_check_step, mops_hb_check_step.
-     rewrite Hhb_check_spec, Hxx0,  hb_check_step.
-     inversion Hfirst_gt.
-     rewrite <- H8, <- H9.
-     eapply assert_le_fail_spec; clarify.
-     rewrite <- leb_le; intro; clarify.
+  induction n; destruct vs1, vs2; intros; subst; try solve [clarify].
+  rewrite hb_check_step, events_hb_check_step, mops_hb_check_step.
+  simpl in Hfirst_gt.
+  destruct (leb n0 n1) eqn: Hle.
+  - exploit IHn.
+    { eauto. }
+    { eauto. }
+    { instantiate (1 := vs1); clarify. }
+    { instantiate (1 := vs2); clarify. }
+    { eauto. }
+    instantiate (3 := upd_env (upd_env G t tmp1 n0) t tmp2 n1).
+    rewrite upd_three, upd_three; auto.
+    rewrite leb_le in *.
+    eapply exec_star_t_trans; eauto.
+    apply assert_le_pass_spec_t; auto; reflexivity.
+  - inversion Hfirst_gt; subst.
+    destruct (le_dec v1 v2); [rewrite <- leb_le in *; clarify|].
+    eapply assert_le_fail_spec_t; auto; reflexivity.
 Qed.
 
 Corollary hb_check_fail_spec: forall n C1 C2 t tmp1 tmp2 P G P1 P2 rest v1 v2
@@ -664,54 +461,37 @@ Corollary hb_check_fail_spec: forall n C1 C2 t tmp1 tmp2 P G P1 P2 rest v1 v2
    (mops_hb_check C1 C2 vs1 vs2 n t)
    None (upd_env (upd_env G t tmp1 v1) t tmp2 v2).
 Proof.
-  destruct n; intros.
-  - destruct vs1, vs2; clarify.
-  - eapply hb_check_fail_spec_n; eauto.
+  intros; eapply exec_t_exec, hb_check_fail_spec_t; eauto.
 Qed.
      
-Lemma hb_check_pass_spec_n: forall n C1 C2 t tmp1 tmp2 P G P1 P2 rest v1 v2 vs1 vs2
- (Hhb_check_spec: P= P1++(t,hb_check C1 C2 (S n) tmp1 tmp2++rest)::P2) 
+Lemma hb_check_pass_spec_t : forall n C1 C2 t tmp1 tmp2 P G P1 P2 rest vs1
+  vs2 (Hhb_check_spec: P= P1++(t,hb_check C1 C2 n tmp1 tmp2++rest)::P2) 
  (Htmp: tmp1 <> tmp2) (Hvs1: length vs1 = n) (Hvs2: length vs2 = n) 
- (Hfirst_gt: first_gt (vs1++[v1]) (vs2++[v2]) = None),
- exec_star (Some P) G (events_hb_check C1 C2 (vs1++[v1]) (vs2++[v2]) t)
-           (mops_hb_check C1 C2 (vs1++[v1]) (vs2++[v2]) (S n) t) 
-           (Some (P1++(t,rest)::P2)) (upd_env (upd_env G t tmp1 v1) t tmp2 v2). 
+ (Hfirst_gt: first_gt vs1 vs2 = None),
+ exec_star_t t (Some P) G (events_hb_check C1 C2 vs1 vs2 t)
+           (mops_hb_check C1 C2 vs1 vs2 n t) (Some (P1++(t,rest)::P2))
+   (upd_env (upd_env G t tmp1 (last vs1 (G t tmp1))) t tmp2 (last vs2 (G t tmp2))).
 Proof.
-  intro n.
-  induction n;intros.
-  -apply empty_list in Hvs1. apply empty_list in Hvs2. clarify.
-   apply assert_le_pass_spec; eauto.
-   rewrite leb_le in cond; auto.
-  -apply nonempty_list in Hvs1;apply nonempty_list in Hvs2;
-  inversion Hvs1; inversion Hvs2; inversion H; inversion H0;
-  inversion H1; inversion H2.
-
-  rewrite H3, H5, list_cons_plus_assoc in Hfirst_gt. 
-  rewrite list_cons_plus_assoc, first_gt_step in Hfirst_gt.
-  
-    destruct (leb x x0) eqn:Hxx0; eauto.
-    +rewrite H3,H5.
-     repeat rewrite list_cons_plus_assoc.
-     rewrite events_hb_check_step, mops_hb_check_step.
-     rewrite Hhb_check_spec, Hxx0,  hb_check_step.
-     eapply exec_star_trans.
-     *apply assert_le_pass_spec; clarify.
-      rewrite leb_le in *; auto.
-     *clarify.
-      assert(Hupd: (upd_env (upd_env G t tmp1 v1) t tmp2 v2)= upd_env (upd_env (upd_env (upd_env G t tmp1 x) t tmp2 x0) t tmp1 v1) t tmp2 v2).
-       symmetry. rewrite upd_assoc. rewrite upd_overwrite.
-       rewrite upd_assoc. rewrite upd_overwrite. eauto.
-       clarify. eauto.
-      rewrite Hupd.
-      eapply IHn; eauto.
-     +rewrite H3,H5.
-      repeat rewrite list_cons_plus_assoc.
-
-      rewrite events_hb_check_step, mops_hb_check_step.
-     rewrite Hhb_check_spec, Hxx0,  hb_check_step.
-     inversion Hfirst_gt.
+  induction n; destruct vs1, vs2; intros; subst; try solve [clarify].
+  { repeat rewrite upd_triv; apply exec_refl_t. }
+  rewrite hb_check_step, events_hb_check_step, mops_hb_check_step.
+  simpl in Hfirst_gt.
+  destruct (leb n0 n1) eqn: Hle; [|clarify].
+  rewrite leb_le in Hle.
+  exploit IHn.
+  { eauto. }
+  { eauto. }
+  { instantiate (1 := vs1); clarify. }
+  { instantiate (1 := vs2); clarify. }
+  { eauto. }
+  instantiate (2 := upd_env (upd_env G t tmp1 n0) t tmp2 n1).
+  rewrite upd_three, upd_three; auto.
+  rewrite upd_old, upd_same, upd_same; auto.
+  do 2 rewrite last_cons'.
+  intro; eapply exec_star_t_trans; eauto.
+  apply assert_le_pass_spec_t; auto; reflexivity.
 Qed.
-
+   
 Lemma hb_check_pass_spec: forall n C1 C2 t tmp1 tmp2 P G P1 P2 rest vs1
   vs2 (Hhb_check_spec: P= P1++(t,hb_check C1 C2 n tmp1 tmp2++rest)::P2) 
  (Htmp: tmp1 <> tmp2) (Hvs1: length vs1 = n) (Hvs2: length vs2 = n) 
@@ -720,17 +500,9 @@ Lemma hb_check_pass_spec: forall n C1 C2 t tmp1 tmp2 P G P1 P2 rest vs1
            (mops_hb_check C1 C2 vs1 vs2 n t) (Some (P1++(t,rest)::P2))
    (upd_env (upd_env G t tmp1 (last vs1 (G t tmp1))) t tmp2 (last vs2 (G t tmp2))).
 Proof.
-  destruct n; intros.
-  - destruct vs1, vs2; clarify.
-    repeat rewrite upd_triv; apply exec_refl.
-  - assert (vs1 <> []) as Hnnil1 by (destruct vs1; clarify).
-    assert (vs2 <> []) as Hnnil2 by (destruct vs2; clarify).
-    rewrite (app_removelast_last 0 Hnnil1) in *.
-    rewrite (app_removelast_last 0 Hnnil2) in *.
-    rewrite app_length in Hvs1, Hvs2; repeat rewrite last_snoc.
-    apply hb_check_pass_spec_n; auto; clarify; omega.
-Qed.    
-   
+  intros; eapply exec_t_exec, hb_check_pass_spec_t; auto.
+Qed.
+
 (* Since everything is a nat, we can use C + t as the t component of C. *)
 
 Class metadata := { C : var; L : var; R : var; W : var; X : var;
@@ -761,35 +533,25 @@ Definition load_handler t x z :=
 Lemma split_app' : forall A (x : A) l, x :: l = [x] ++ l.
 Proof. auto. Qed.
 
-Opaque hb_check.
-Opaque move.
-
-Lemma load_handler_norace_spec_n: forall n x t P G P1 P2 rest v1 v2 vs1 vs2
- (Hload_handler_spec: P= P1++(t,load_handler t x (S n)++rest)::P2) 
- (Hvs1: length vs1 = n) (Hvs2: length vs2 = n) 
- (Hfirst_gt: first_gt (vs1++[v1]) (vs2++[v2]) = None) v,
- exec_star (Some P) G 
-           (acq t (X + x) :: events_hb_check (W + x) (C + t) (vs1++[v1]) (vs2++[v2]) t ++ events_move (C+t) (R+x) t)
-           (Acq t (X + x) :: mops_hb_check (W + x) (C + t) (vs1++[v1]) (vs2++[v2]) (S n) t ++ mops_move (C+t,t) (R+x, t) t v)
-           (Some (P1++(t,rest)::P2)) (upd_env (upd_env G t tmp1 v) t tmp2 v2).
+Lemma load_handler_norace_spec_t : forall n x t P G P1 P2 rest
+  vs1 vs2 (Hload_handler_spec: P = P1 ++ (t, load_handler t x n ++ rest) :: P2)   (Hvs1 : length vs1 = n)
+  (Hvs2 : length vs2 = n) (Hfirst_gt : first_gt vs1 vs2 = None) v,
+  exec_star_t t (Some P) G
+    (acq t (X + x) :: events_hb_check (W + x) (C + t) vs1 vs2 t ++ events_move (C + t) (R + x) t)
+    (Acq t (X + x) :: mops_hb_check (W + x) (C + t) vs1 vs2 n t ++ mops_move (C + t, t) (R + x, t) t v)
+    (Some (P1 ++ (t, rest) :: P2)) (upd_env (upd_env G t tmp1 v) t tmp2 (last vs2 (G t tmp2))).
 Proof.
   clarify.
-  eapply (exec_step' (exec_lock _ _ _ _ _ _ eq_refl)); clarify.
-  eapply exec_star_trans.
-  rewrite <- app_assoc; apply hb_check_pass_spec_n; auto.
-  rewrite upd_assoc; auto.
-  setoid_rewrite upd_assoc at 2; auto.
-  setoid_rewrite <- (upd_overwrite _ _ _ v1) at 3; apply move_spec; auto.
+  eapply exec_step_t'.
+  { apply exec_lock; eauto. }
+  rewrite <- app_assoc.
+  eapply exec_star_t_trans.
+  - eapply hb_check_pass_spec_t; try apply Hfirst_gt; eauto.
+  - exploit move_spec_t; eauto.
+    rewrite upd_three; eauto.
+  - auto. 
+  - auto.
 Qed.
-
-(* updates to different locals don't interfere with each other*)
-Lemma upd_old : forall G t1 a1 v1 t2 a2 (Ha : a1 <> a2),
-  upd_env G t1 a1 v1 t2 a2 = G t2 a2.
-Proof.
-  intros; unfold upd_env, upd; clarify.
-Qed.
-
-Transparent hb_check.
 
 Corollary load_handler_norace_spec: forall n x t P G P1 P2 rest
   vs1 vs2 (Hload_handler_spec: P = P1 ++ (t, load_handler t x n ++ rest) :: P2)   (Hvs1 : length vs1 = n)
@@ -799,37 +561,25 @@ Corollary load_handler_norace_spec: forall n x t P G P1 P2 rest
     (Acq t (X + x) :: mops_hb_check (W + x) (C + t) vs1 vs2 n t ++ mops_move (C + t, t) (R + x, t) t v)
     (Some (P1 ++ (t, rest) :: P2)) (upd_env (upd_env G t tmp1 v) t tmp2 (last vs2 (G t tmp2))).
 Proof.
-  intros; destruct n; clarify.
-  - destruct vs1, vs2; clarify.
-    assert (upd_env G t tmp1 v t tmp2 = G t tmp2) as Heq
-      by (apply upd_old; auto).
-    rewrite <- Heq, upd_triv.
-    eapply (exec_step' (exec_lock _ _ _ _ _ _ eq_refl)); clarify.
-    apply move_spec; auto.
-  - assert (vs1 <> []) as Hnnil1 by (destruct vs1; clarify).
-    assert (vs2 <> []) as Hnnil2 by (destruct vs2; clarify).
-    rewrite (app_removelast_last 0 Hnnil1) in *.
-    rewrite (app_removelast_last 0 Hnnil2) in *.
-    rewrite app_length in Hvs1, Hvs2; clarify.
-    rewrite last_snoc; apply load_handler_norace_spec_n; auto; omega.
+  intros; eapply exec_t_exec, load_handler_norace_spec_t; auto.
 Qed.
 
-Opaque hb_check.
-
-Lemma load_handler_race_spec_n: forall n x t P G P1 P2 rest v1 v2 vs1 vs2
- (Hload_handler_spec: P= P1++(t,load_handler t x (S n)++rest)::P2) 
- (Htmp: tmp1 <> tmp2) (Hvs1: length vs1 = S n) (Hvs2: length vs2 = S n) 
- (Hfirst_gt: first_gt vs1 vs2 = Some (v1,v2)),
- exec_star (Some P) G (acq t (X + x) :: events_hb_check (W + x) (C + t) vs1 vs2 t)
-           (Acq t (X + x) :: mops_hb_check (W + x) (C + t) vs1 vs2 (S n) t) 
+Lemma load_handler_race_spec_t : forall n x t P G P1 P2 rest
+  vs1 vs2 (Hload_handler_spec: P = P1++(t,load_handler t x n++
+  rest)::P2) (Hvs1: length vs1 = n) (Hvs2: length vs2 = n) 
+  v1 v2 (Hfirst_gt: first_gt vs1 vs2 = Some (v1,v2)),
+ exec_star_t t (Some P) G (acq t (X + x) :: events_hb_check (W + x) (C + t) vs1 vs2 t)
+           (Acq t (X + x) :: mops_hb_check (W + x) (C + t) vs1 vs2 n t) 
            None (upd_env (upd_env G t tmp1 v1) t tmp2 v2).
 Proof.
-  intros; subst.
-  unfold load_handler; simpl.
-  eapply (exec_step' (exec_lock _ _ _ _ _ _ eq_refl)); clarify.
-  eapply hb_check_fail_spec_n; eauto.
-  rewrite <- app_assoc; eauto.
-Qed.
+  clarify.
+  eapply exec_step_t'.
+  { apply exec_lock; eauto. }
+  rewrite <- app_assoc.
+  eapply hb_check_fail_spec_t; try apply Hfirst_gt; eauto.
+  - auto.
+  - auto.
+Qed.  
 
 Corollary load_handler_race_spec: forall n x t P G P1 P2 rest
   vs1 vs2 (Hload_handler_spec: P = P1++(t,load_handler t x n++
@@ -839,59 +589,32 @@ Corollary load_handler_race_spec: forall n x t P G P1 P2 rest
            (Acq t (X + x) :: mops_hb_check (W + x) (C + t) vs1 vs2 n t) 
            None (upd_env (upd_env G t tmp1 v1) t tmp2 v2).
 Proof.
-  destruct n; intros.
-  - destruct vs1, vs2; clarify.
-  - eapply load_handler_race_spec_n; eauto.
+  intros; eapply exec_t_exec, load_handler_race_spec_t; eauto.
 Qed.
 
 Definition store_handler t x z :=
   Lock (X + x) :: hb_check (W + x) (C + t) z tmp1 tmp2 ++
   hb_check (R + x) (C + t) z tmp1 tmp2 ++
   move (C + t, t) (W + x, t) tmp1.
-Lemma store_handler_race_waw_spec_n: forall n x t P G P1 P2 rest v1 v2 vs1 vs2
- (Hstore_handler_spec: P= P1++(t,store_handler t x (S n)++rest)::P2) 
- (Hvs1: length vs1 = S n) (Hvs2: length vs2 = S n) 
+
+Lemma store_handler_race_waw_spec_t : forall n x t P G P1 P2 rest v1 v2 vs1 vs2
+ (Hstore_handler_spec: P= P1++(t,store_handler t x  n++rest)::P2) 
+ (Hvs1: length vs1 = n) (Hvs2: length vs2 = n) 
  (Hfirst_gt: first_gt vs1 vs2 = Some (v1,v2)),
- exec_star (Some P) G (acq t (X + x) :: events_hb_check (W + x) (C + t) vs1 vs2 t)
-           (Acq t (X + x) :: mops_hb_check (W + x) (C + t) vs1 vs2 (S n) t) 
+ exec_star_t t (Some P) G (acq t (X + x) :: events_hb_check (W + x) (C + t) vs1 vs2 t)
+           (Acq t (X + x) :: mops_hb_check (W + x) (C + t) vs1 vs2 n t) 
            None (upd_env (upd_env G t tmp1 v1) t tmp2 v2). 
 Proof.
-  intros.
-  unfold store_handler in Hstore_handler_spec; clarify.
-  eapply (exec_step' (exec_lock _ _ _ _ _ _ eq_refl)); clarify.
-  eapply hb_check_fail_spec_n; eauto.
-  rewrite <- app_assoc; eauto.
+  clarify.
+  eapply exec_step_t'.
+  { apply exec_lock; eauto. }
+  rewrite <- app_assoc.
+  eapply hb_check_fail_spec_t; try apply Hfirst_gt; eauto.
+  - auto.
+  - auto.
 Qed.
 
-Lemma store_handler_race_war_spec_n: forall n x t P G P1 P2 rest ve1 ve2 ve3 v2 v3 vs1 vs2 vs3
- (Hstore_handler_spec: P= P1++(t,store_handler t x (S n)++rest)::P2) 
- (Hvs1: length vs1 = n) (Hvs2: length vs2 = n) (Hvs3: length vs3 = n) 
- (Hfirst_gt12: first_gt (vs1++[ve1]) (vs2++[ve2]) = None)
- (Hfirst_gt32: first_gt (vs3++[ve3]) (vs2++[ve2]) = Some (v3,v2)),
-
- exec_star (Some P) G 
-           (acq t (X + x) :: events_hb_check (W + x) (C + t) (vs1++[ve1]) (vs2++[ve2]) t ++
-            events_hb_check (R + x) (C + t) (vs3++[ve3]) (vs2++[ve2]) t)
-           (Acq t (X + x) :: mops_hb_check (W + x) (C + t) (vs1++[ve1]) (vs2++[ve2]) (S n) t ++
-            mops_hb_check (R + x) (C + t) (vs3++[ve3]) (vs2++[ve2]) (S n) t) 
-           None (upd_env (upd_env G t tmp1 v3) t tmp2 v2). 
-Proof.
-  intros.
-  unfold store_handler in Hstore_handler_spec; clarify.
-  eapply (exec_step' (exec_lock _ _ _ _ _ _ eq_refl)); clarify.
-  rewrite <- app_assoc; eapply exec_star_trans.
-  - apply hb_check_pass_spec_n; try (apply Hfirst_gt12); eauto.
-  - assert(Hupd: upd_env (upd_env G t tmp1 v3) t tmp2 v2 =
-                 upd_env (upd_env (upd_env (upd_env G t tmp1 ve1) t tmp2 ve2) t tmp1 v3) t tmp2 v2).
-    { symmetry. rewrite upd_assoc. rewrite upd_overwrite. rewrite upd_assoc. rewrite upd_overwrite. eauto.
-      eauto.
-      eauto. }
-    rewrite <- app_assoc, Hupd.
-    eapply hb_check_fail_spec_n; eauto;
-      clarify; rewrite app_length; rewrite plus_comm; auto.
-Qed.
-
-Lemma store_handler_race_waw_spec: forall n x t P G P1 P2 rest v1 v2 vs1 vs2
+Corollary store_handler_race_waw_spec: forall n x t P G P1 P2 rest v1 v2 vs1 vs2
  (Hstore_handler_spec: P= P1++(t,store_handler t x  n++rest)::P2) 
  (Hvs1: length vs1 = n) (Hvs2: length vs2 = n) 
  (Hfirst_gt: first_gt vs1 vs2 = Some (v1,v2)),
@@ -899,11 +622,34 @@ Lemma store_handler_race_waw_spec: forall n x t P G P1 P2 rest v1 v2 vs1 vs2
            (Acq t (X + x) :: mops_hb_check (W + x) (C + t) vs1 vs2 n t) 
            None (upd_env (upd_env G t tmp1 v1) t tmp2 v2). 
 Proof.
-  destruct n; intros.
-  -destruct vs1, vs2; clarify.
-  -eapply store_handler_race_waw_spec_n; eauto.
+  intros; eapply exec_t_exec, store_handler_race_waw_spec_t; eauto.
 Qed.
- 
+
+Lemma store_handler_race_war_spec_t : forall n x t P G P1 P2 rest v2 v3 vs1 vs2 vs3
+ (Hstore_handler_spec: P= P1++(t,store_handler t x n ++rest)::P2) 
+ (Hvs1: length vs1 = n) (Hvs2: length vs2 = n) (Hvs3: length vs3 = n) 
+ (Hfirst_gt12: first_gt vs1 vs2 = None)
+ (Hfirst_gt32: first_gt vs3 vs2 = Some (v3,v2)),
+ exec_star_t t (Some P) G 
+           (acq t (X + x) :: events_hb_check (W + x) (C + t) vs1 vs2 t ++
+            events_hb_check (R + x) (C + t) vs3 vs2 t)
+           (Acq t (X + x) :: mops_hb_check (W + x) (C + t) vs1 vs2 n t ++
+            mops_hb_check (R + x) (C + t) vs3 vs2 n t) 
+           None (upd_env (upd_env G t tmp1 v3) t tmp2 v2). 
+Proof.
+  clarify.
+  eapply exec_step_t'.
+  { apply exec_lock; eauto. }
+  repeat rewrite <- app_assoc.
+  eapply exec_star_t_trans; [apply hb_check_pass_spec_t; try apply Hfirst_gt12;
+                            eauto|].
+  exploit hb_check_fail_spec_t; try apply Hfirst_gt32; eauto.
+  instantiate (5 := upd_env (upd_env G t tmp1 (last vs1 (G t tmp1))) t tmp2
+        (last vs2 (G t tmp2))).
+  rewrite upd_three, upd_three; eauto.
+  - auto.
+  - auto.
+Qed.
 
 Lemma store_handler_race_war_spec: forall n x t P G P1 P2 rest v2 v3 vs1 vs2 vs3
  (Hstore_handler_spec: P= P1++(t,store_handler t x n ++rest)::P2) 
@@ -918,54 +664,45 @@ Lemma store_handler_race_war_spec: forall n x t P G P1 P2 rest v2 v3 vs1 vs2 vs3
             mops_hb_check (R + x) (C + t) vs3 vs2 n t) 
            None (upd_env (upd_env G t tmp1 v3) t tmp2 v2). 
 Proof.
-  destruct n; intros.
-  -destruct vs1, vs2, vs3; clarify.
-  -assert(Hves: exists ve1 ve2 ve3 vss1 vss2 vss3, vs1=vss1++[ve1]/\ vs2=vss2++[ve2] /\ vs3=vss3++[ve3]).
-     destruct vs1, vs2, vs3; clarify.
-     do 6 eexists.
-     instantiate(1:=last (n2::vs3) n2). instantiate (1:=removelast (n2::vs3)).
-     instantiate(1:=last (n1::vs2) n1). instantiate (1:=removelast (n1::vs2)).
-     instantiate(1:=last (n0::vs1) n0). instantiate (1:=removelast (n0::vs1)).
-     repeat rewrite <- app_removelast_last; clarify.
-    inversion Hves; clarify.
-    eapply store_handler_race_war_spec_n; eauto. 
-    +instantiate(1:=P2). instantiate(1:=rest). instantiate(1:=P1). auto.
-    + rewrite app_length in *. simpl in *. omega.
-    + rewrite app_length in *. simpl in *. omega.
-    + rewrite app_length in *. simpl in *. omega.
+  intros; eapply exec_t_exec, store_handler_race_war_spec_t; eauto.
 Qed.
 
-Lemma store_handler_norace_spec_n: forall n x t P G P1 P2 rest v1 v2 v3 vs1 vs2 vs3
- (Hstore_handler_spec: P= P1++(t,store_handler t x (S n)++rest)::P2) 
- (Hvs1: length vs1 = n) (Hvs2: length vs2 = n) (Hvs3: length vs3 =n) 
- (Hfirst_gt12: first_gt (vs1++[v1]) (vs2++[v2]) = None)
- (Hfirst_gt32: first_gt (vs3++[v3]) (vs2++[v2]) = None) v,
- exec_star (Some P) G 
-           (acq t (X + x) :: events_hb_check (W + x) (C + t) (vs1++[v1]) (vs2++[v2]) t ++ 
-            events_hb_check (R + x) (C + t) (vs3++[v3]) (vs2++[v2]) t ++               
-            events_move (C+t) (W+x) t)
-           (Acq t (X + x) :: mops_hb_check (W + x) (C + t) (vs1++[v1]) (vs2++[v2]) (S n) t ++ 
-            mops_hb_check (R + x) (C + t) (vs3++[v3]) (vs2++[v2]) (S n) t ++
-            mops_move (C+t,t) (W+x, t) t v) 
-           (Some (P1++(t,rest)::P2)) (upd_env (upd_env G t tmp1 v) t tmp2 v2).
+(* up *)
+Lemma last_last : forall A (d : A) l, last l (last l d) = last l d.
 Proof.
-  intros.
-  unfold store_handler in Hstore_handler_spec; clarify.
-  eapply (exec_step' (exec_lock _ _ _ _ _ _ eq_refl)); clarify.
-  rewrite <- app_assoc; eapply exec_star_trans.
-  - apply hb_check_pass_spec_n; try (apply Hfirst_gt12); eauto.
-  - repeat rewrite <- app_assoc.
-    eapply exec_star_trans.
-    + apply hb_check_pass_spec_n; try (apply Hfirst_gt32); eauto.
-    + do 2 (rewrite upd_assoc, upd_overwrite; auto).
-      rewrite upd_assoc; auto.
-      setoid_rewrite upd_assoc at 2; auto.
-      setoid_rewrite <- (upd_overwrite _ _ _ v3) at 3; apply move_spec; auto.
+  destruct l; clarify.
+  apply last_def; clarify.
 Qed.
 
-
-
-Transparent hb_check.
+Lemma store_handler_norace_spec_t : forall n x t P G P1 P2 rest
+  vs1 vs2 vs3 (Hstore_handler_spec: P = P1 ++ (t, store_handler t x n
+  ++ rest) :: P2) (Hvs1 : length vs1 = n)
+  (Hvs2 : length vs2 = n) (Hvs3: length vs3 = n) (Hfirst_gt12 : first_gt vs1 vs2 = None) (Hfirst_gt32: first_gt vs3 vs2 = None) v,
+  exec_star_t t (Some P) G
+    (acq t (X + x) :: events_hb_check (W + x) (C + t) vs1 vs2 t ++ 
+     events_hb_check (R + x) (C + t) vs3 vs2 t ++
+     events_move (C + t) (W + x) t)
+    (Acq t (X + x) :: mops_hb_check (W + x) (C + t) vs1 vs2 n t ++
+     mops_hb_check (R + x) (C + t) vs3 vs2 n t ++
+     mops_move (C + t, t) (W + x, t) t v )
+    (Some (P1 ++ (t, rest) :: P2)) (upd_env (upd_env G t tmp1 v) t tmp2 (last vs2 (G t tmp2))).
+Proof.
+  clarify.
+  eapply exec_step_t'.
+  { apply exec_lock; eauto. }
+  repeat rewrite <- app_assoc.
+  eapply exec_star_t_trans; [apply hb_check_pass_spec_t; try apply Hfirst_gt12;
+                            eauto|].
+  eapply exec_star_t_trans; [apply hb_check_pass_spec_t; try apply Hfirst_gt32;
+                            eauto|].
+  repeat rewrite upd_three; auto.
+  rewrite upd_old, upd_same, upd_same; auto.
+  repeat rewrite last_last.
+  exploit move_spec_t; eauto.
+  rewrite upd_three; eauto.
+  - auto.
+  - auto.
+Qed.
 
 Corollary store_handler_norace_spec: forall n x t P G P1 P2 rest
   vs1 vs2 vs3 (Hstore_handler_spec: P = P1 ++ (t, store_handler t x n
@@ -980,126 +717,197 @@ Corollary store_handler_norace_spec: forall n x t P G P1 P2 rest
      mops_move (C + t, t) (W + x, t) t v )
     (Some (P1 ++ (t, rest) :: P2)) (upd_env (upd_env G t tmp1 v) t tmp2 (last vs2 (G t tmp2))).
 Proof.
-  intros; destruct n; clarify.
-  - destruct vs1, vs2, vs3; clarify.
-    assert (upd_env G t tmp1 v t tmp2 = G t tmp2) as Heq
-      by (apply upd_old; auto).
-    rewrite <- Heq, upd_triv.
-    eapply (exec_step' (exec_lock _ _ _ _ _ _ eq_refl)); clarify.
-    apply move_spec; auto.
-  - assert (vs1 <> []) as Hnnil1 by (destruct vs1; clarify).
-    assert (vs2 <> []) as Hnnil2 by (destruct vs2; clarify).
-    assert (vs3 <> []) as Hnnil3 by (destruct vs3; clarify).
-    rewrite (app_removelast_last 0 Hnnil1) in *.
-    rewrite (app_removelast_last 0 Hnnil2) in *.
-    rewrite (app_removelast_last 0 Hnnil3) in *.
-    rewrite app_length in Hvs1, Hvs2, Hvs3; clarify.
-    rewrite last_snoc; apply store_handler_norace_spec_n; auto; omega.
+  intros; eapply exec_t_exec, store_handler_norace_spec_t; auto.
 Qed.
    
 Definition lock_handler t l z :=
   max_vc (L+l) (C+t) z tmp1 tmp2.
 
-Lemma lock_handler_spec_n : forall n t l P G P1 P2 rest v1 v2 vss1 vss2
+(* up! *)
+Lemma last_single : forall A (x d : A), last [x] d = x.
+Proof. auto. Qed.
 
-(Hmax_vc: P=P1++(t, lock_handler t l (S n) ++ rest)::P2) (Hvs1: length vss1=n) (Hvs2: length vss2=n),
- exec_star (Some P) G
-          (events_max_vc (L+l) (C+t) t (S n)) (mops_max_vc (L+l) (C+t) (vss1++[v1]) (vss2++[v2]) t (S n)) (Some (P1++(t,rest)::P2)) (upd_env (upd_env G t tmp1 v1) t tmp2 (Peano.max v1 v2)).  
+Lemma lock_handler_spec_t : forall n t l P G P1 P2 rest vs1 vs2 v
+  (HP : P = P1 ++ (t, lock_handler t l n ++ rest) :: P2)
+  (Hlen1 : length vs1 = n) (Hlen2 : length vs2 = n) (Hn : n <> 0),
+  exec_star_t t (Some P) G (events_max_vc (L + l) (C + t) t n)
+    (mops_max_vc (L + l) (C + t) vs1 vs2 t n) (Some (P1 ++ (t, rest) :: P2))
+    (upd_env (upd_env G t tmp1 (last vs1 0)) t tmp2
+       (Peano.max (last vs1 v) (last vs2 v))).
 Proof.
-  intros.
-  apply max_vc_spec_n; eauto.
-Qed.
+  induction n; clarify.
+  destruct vs1, vs2; clarify.
+  eapply exec_step_t'; eauto.
+  { apply exec_load; eauto. }
+  eapply exec_step_t'; eauto.
+  { apply exec_load; eauto. }
+  eapply exec_step_t'; eauto.
+  { apply exec_assign; eauto. }
+  eapply exec_step_t'; eauto.
+  { apply exec_store; eauto. }
+  instantiate (1 := mops_max_vc (L + l) (C + t) vs1 vs2 t n).
+  instantiate (1 := events_max_vc (L + l) (C + t) t n).
+  rewrite upd_overwrite.
+  destruct (eq_dec n 0).
+  - clarify.
+    destruct vs1; clarify.
+    repeat rewrite last_single.
+    rewrite upd_old, upd_same, upd_same; auto.
+    apply exec_refl_t.
+  - repeat rewrite last_cons; try solve [intro; clarify; omega].
+    exploit IHn.
+    { eauto. }
+    { instantiate (1 := vs1); auto. }
+    { instantiate (1 := vs2); auto. }
+    { auto. }
+    instantiate (5 := upd_env (upd_env G t tmp1 n0) t tmp2
+        (eval (upd_env (upd_env G t tmp1 n0) t tmp2 n1 t)
+           (Max (V tmp1) (V tmp2)))).
+    setoid_rewrite upd_assoc at 2; auto.
+    rewrite upd_overwrite.
+    setoid_rewrite upd_assoc at 2; auto.
+    rewrite upd_overwrite; eauto.
+  - auto.
+  - simpl.
+    rewrite upd_overwrite, upd_same, upd_same.
+    rewrite upd_assoc, upd_same; auto.
+Qed.  
 
-Lemma lock_handler_spec : forall n t l P G P1 P2 rest vs1 vs2 v
-
-(Hmax_vc: P=P1++(t, lock_handler t l n ++ rest)::P2) (Htmp: tmp1 <> tmp2) (Hvs1: length vs1=n) (Hvs2: length vs2=n) (Ht: t<n),
- exec_star (Some P) G
-          (events_max_vc (L+l) (C+t) t n) (mops_max_vc (L+l) (C+t) (vs1) (vs2) t  n) (Some (P1++(t,rest)::P2)) (upd_env (upd_env G t tmp1 (last vs1 0)) t tmp2 (Peano.max (last vs1 v) (last vs2 v))).  
+Corollary lock_handler_spec : forall n t l P G P1 P2 rest vs1 vs2 v
+  (HP : P = P1 ++ (t, lock_handler t l n ++ rest) :: P2)
+  (Hlen1 : length vs1 = n) (Hlen2 : length vs2 = n) (Hn : n <> 0),
+  exec_star (Some P) G (events_max_vc (L + l) (C + t) t n)
+    (mops_max_vc (L + l) (C + t) vs1 vs2 t n) (Some (P1 ++ (t, rest) :: P2))
+    (upd_env (upd_env G t tmp1 (last vs1 0)) t tmp2
+       (Peano.max (last vs1 v) (last vs2 v))).
 Proof.
-  
-  intros; destruct n.
-  - inversion Ht.
-  -assert(vs1 <>[]) as Hnnil1 by (destruct vs1; clarify).
-   assert(vs2 <>[]) as Hnnil2 by (destruct vs2; clarify).
-  
-   rewrite (app_removelast_last v Hnnil1) in *.
-   rewrite (app_removelast_last v Hnnil2) in *.
-   rewrite app_length in Hvs1, Hvs2.
-   repeat rewrite last_snoc.
-   apply lock_handler_spec_n with (vss1:=removelast vs1) (vss2:=removelast vs2) (v1:=last vs1 v) (v2:= last vs2 v).
-   eauto.
-   eauto.
-   clarify. omega.
-   clarify. omega.
+  intros; eapply exec_t_exec, lock_handler_spec_t; auto.
 Qed.
-
 
 Definition unlock_handler t m z tmp :=
   set_vc (C + t) (L + m) z tmp ++ inc_vc t (C + t) tmp.
 
-
-
-(* mod? *)
-Lemma unlock_handler_spec_n : forall n u tmp P G P1 P2 t rest v vss vt
-(Hset_vc: P=P1++(t, unlock_handler t u (S n) tmp++ rest)::P2) (Hvs: length vss=n),
- exec_star (Some P) G
-          (events_set_vc (C+t)(L+u) (S n) t++(events_inc_vc (C+t) t)) (mops_set_vc (C+t) (L+u) (S n) t (vss++[v])++ (mops_inc_vc (C+t) vt t)) (Some (P1++(t,rest)::P2)) (upd_env G t tmp (vt+1)).
+Lemma unlock_handler_spec_t : forall n u tmp P G P1 P2 t rest vss vt
+(Hset_vc: P=P1++(t, unlock_handler t u n tmp++ rest)::P2) (Hvs: length vss=n),
+ exec_star_t t (Some P) G
+          (events_set_vc (C+t)(L+u) n t++(events_inc_vc (C+t) t)) (mops_set_vc (C+t) (L+u) n t vss++ (mops_inc_vc (C+t) vt t)) (Some (P1++(t,rest)::P2)) (upd_env G t tmp (vt+1)).
 Proof.
-  intros.
-  unfold unlock_handler in Hset_vc.
-  apply exec_star_trans with (P':=P1++(t,inc_vc t (C+t) tmp++rest)::P2) (G':=upd_env G t tmp v). 
-  -eapply set_vc_spec_n;eauto.
-   rewrite app_assoc. eauto.
-  -assert(Hoverwrite:upd_env G t tmp (vt+1) =upd_env (upd_env G t tmp v) t tmp (vt+1)).
-   rewrite <- upd_overwrite with (v1:=v). eauto.
-   rewrite Hoverwrite.
-   apply inc_vc_spec. eauto.
+  clarify.
+  setoid_rewrite <- app_assoc.
+  eapply exec_star_t_trans; [apply set_vc_spec_t; eauto|].
+  exploit inc_vc_spec_t; eauto.
+  rewrite upd_overwrite; eauto.
 Qed.
 
+Corollary unlock_handler_spec : forall n u tmp P G P1 P2 t rest vss vt
+(Hset_vc: P=P1++(t, unlock_handler t u n tmp++ rest)::P2) (Hvs: length vss=n),
+ exec_star (Some P) G
+          (events_set_vc (C+t)(L+u) n t++(events_inc_vc (C+t) t)) (mops_set_vc (C+t) (L+u) n t vss++ (mops_inc_vc (C+t) vt t)) (Some (P1++(t,rest)::P2)) (upd_env G t tmp (vt+1)).
+Proof.
+  intros; eapply exec_t_exec, unlock_handler_spec_t; auto.
+Qed.
 
 Definition spawn_handler t l z :=
   max_vc (C + t) (C+l) z tmp1 tmp2 ++ inc_vc t (C + t) tmp1.
 
-Lemma spawn_handler_spec_n : forall n l P G P1 P2 t rest v1 vss1 v2 vss2 vt
-(Hset_vc: P=P1++(t, spawn_handler t l (S n) ++ rest)::P2) (Hvs1: length vss1=n) (Hvs2: length vss2=n) (Htmp: tmp1<>tmp2),
- exec_star (Some P) G
-          (events_max_vc (C+t)(C+l) t (S n)++(events_inc_vc (C+t) t)) (mops_max_vc (C+t) (C+l )(vss1++[v1]) (vss2++[v2]) t (S n) ++ (mops_inc_vc (C+t) vt t)) (Some (P1++(t,rest)::P2)) (upd_env (upd_env G t tmp2 (Peano.max v1 v2)) t tmp1 (vt+1)).
+Lemma spawn_handler_spec_t : forall n l P G P1 P2 t rest vss1 vss2 vt
+(Hset_vc: P=P1++(t, spawn_handler t l n ++ rest)::P2) (Hvs1: length vss1=n) (Hvs2: length vss2=n) (Htmp: tmp1<>tmp2),
+ exec_star_t t (Some P) G
+          (events_max_vc (C+t)(C+l) t n++(events_inc_vc (C+t) t)) (mops_max_vc (C+t) (C+l) vss1 vss2 t n ++ (mops_inc_vc (C+t) vt t)) (Some (P1++(t,rest)::P2)) (upd_env (upd_env G t tmp2 (last (map (fun x => Peano.max (fst x) (snd x))
+  (combine vss1 vss2)) (G t tmp2))) t tmp1 (vt+1)).
 Proof.
-  intros.
-  apply exec_star_trans with (P':=P1++(t,inc_vc t (C+t) tmp1++rest)::P2) (G':=upd_env (upd_env G t tmp1 v1) t tmp2 (Peano.max v1 v2)).
-  -apply max_vc_spec_n. rewrite app_assoc. eauto. auto. auto. auto.
-  -assert(Hoverwrite: upd_env (upd_env G t tmp2 (Peano.max v1 v2)) t tmp1 (vt+1) = upd_env (upd_env (upd_env G t tmp1 v1) t tmp2 (Peano.max v1 v2)) t tmp1 (vt+1)).
-    symmetry. rewrite upd_assoc. rewrite upd_overwrite. rewrite upd_assoc. eauto.
-    eauto. eauto.
-   rewrite Hoverwrite.
-   apply inc_vc_spec. 
-   eauto.
+  clarify.
+  setoid_rewrite <- app_assoc.
+  eapply exec_star_t_trans; [apply max_vc_spec_t; eauto|].
+  exploit inc_vc_spec_t; eauto.
+  instantiate (4 := upd_env (upd_env G t tmp1 (last vss1 (G t tmp1))) t tmp2
+    (last (map (fun x => Peano.max (fst x) (snd x)) (combine vss1 vss2))
+          (G t tmp2))).
+  rewrite upd_three; auto.
+  rewrite upd_assoc with (v1 := vt + 1); eauto.
 Qed.
 
+Lemma spawn_handler_spec : forall n l P G P1 P2 t rest vss1 vss2 vt
+(Hset_vc: P=P1++(t, spawn_handler t l n ++ rest)::P2) (Hvs1: length vss1=n) (Hvs2: length vss2=n) (Htmp: tmp1<>tmp2),
+ exec_star (Some P) G
+          (events_max_vc (C+t)(C+l) t n++(events_inc_vc (C+t) t)) (mops_max_vc (C+t) (C+l) vss1 vss2 t n ++ (mops_inc_vc (C+t) vt t)) (Some (P1++(t,rest)::P2)) (upd_env (upd_env G t tmp2 (last (map (fun x => Peano.max (fst x) (snd x))
+  (combine vss1 vss2)) (G t tmp2))) t tmp1 (vt+1)).
+Proof.
+  intros; eapply exec_t_exec, spawn_handler_spec_t; auto.
+Qed.
 
-
-
-   
-    
 
 Definition wait_handler t u z :=
   max_vc (C + u) (C + t) z tmp1 tmp2
          ++inc_vc u (C + u) tmp1.
 
-(* The instrumentation pass is provided locations to store each of the
-   race detection state components. *)
-Lemma wait_handler_spec_n : forall n t u P G P1 P2 rest v1 v2 vss1 vss2 v
-
-(Hmax_vc: P=P1++(t, wait_handler t u (S n) ++ rest)::P2) (Hvs1: length vss1=n) (Hvs2: length vss2=n),
- exec_star (Some P) G
-          (events_max_vc (C+u) (C+t) t (S n)++ events_inc_vc (C+u) t) (mops_max_vc (C+u) (C+t) (vss1++[v1]) (vss2++[v2]) t (S n) ++ mops_inc_vc' (C+u) v t u) (Some (P1++(t,rest)::P2)) (upd_env (upd_env G t tmp2 (Peano.max v1 v2)) t tmp1 (v+1)).  
+Lemma wait_handler_spec_t : forall n t u P G P1 P2 rest vs1 vs2 v
+  (HP : P = P1 ++ (t, wait_handler t u n ++ rest) :: P2)
+  (Hlen1 : length vs1 = n) (Hlen2 : length vs2 = n) (Hn : n <> 0),
+  exec_star_t t (Some P) G
+    (events_max_vc (C + u) (C + t) t n ++ events_inc_vc (C + u) t)
+    (mops_max_vc (C + u) (C + t) vs1 vs2 t n ++ mops_inc_vc' (C + u) v t u)
+    (Some (P1 ++ (t, rest) :: P2))
+    (upd_env (upd_env G t tmp2 (Peano.max (last vs1 0) (last vs2 0)))
+             t tmp1 (v + 1)).
 Proof.
-  intros.
-  eapply exec_star_trans; eauto. 
-  -eapply max_vc_spec_n; eauto. unfold wait_handler in Hmax_vc. rewrite <- app_assoc in Hmax_vc. eauto.
-  -assert(Hoverwrite: upd_env (upd_env G t tmp2 (Peano.max v1 v2)) t tmp1 (v+1) = upd_env (upd_env (upd_env G t tmp1 v1) t tmp2 (Peano.max v1 v2)) t tmp1 (v+1)).
-   { symmetry. rewrite upd_assoc; auto. rewrite upd_overwrite. rewrite upd_assoc; auto. }
-   rewrite Hoverwrite.  apply inc_vc_spec'. auto.
+  induction n; clarify.
+  destruct vs1, vs2; clarify.
+  eapply exec_step_t'; eauto.
+  { apply exec_load; eauto. }
+  eapply exec_step_t'; eauto.
+  { apply exec_load; eauto. }
+  eapply exec_step_t'; eauto.
+  { apply exec_assign; eauto. }
+  rewrite upd_overwrite; simpl.
+  rewrite upd_same, upd_old, upd_same; auto.
+  eapply exec_step_t'; eauto.
+  { apply exec_store; eauto. }
+  instantiate (1 := mops_max_vc (C + u) (C + t) vs1 vs2 t n ++
+    mops_inc_vc' (C + u) v t u).
+  instantiate (1 := events_max_vc (C + u) (C + t) t n ++
+    events_inc_vc (C + u) t).
+  destruct (eq_dec n 0).
+  - destruct vs1, vs2; clarify.
+    repeat rewrite last_single.
+    eapply exec_step_t'; eauto.
+    { apply exec_load; eauto. }
+    eapply exec_step_t'; eauto.
+    { apply exec_assign; eauto. }
+    simpl; eapply exec_step_t'; eauto.
+    { apply exec_store; eauto. }
+    repeat rewrite upd_three; auto.
+    rewrite upd_old, upd_same, upd_assoc; auto.
+    apply exec_refl_t.
+    + auto.
+    + simpl.
+      repeat rewrite upd_same; auto.
+  - repeat rewrite last_cons; try solve [intro; clarify; omega].
+    exploit IHn.
+    { eauto. }
+    { instantiate (1 := vs1); auto. }
+    { instantiate (1 := vs2); auto. }
+    { auto. }
+    instantiate (4 := upd_env (upd_env G t tmp1 n0) t tmp2 (Peano.max n0 n1)).
+    rewrite upd_overwrite.
+    rewrite upd_three; auto.
+    setoid_rewrite upd_assoc at 2; eauto.
+  - auto.
+  - simpl.
+    rewrite upd_same; auto.
+Qed.  
+
+Corollary wait_handler_spec : forall n t u P G P1 P2 rest vs1 vs2 v
+  (HP : P = P1 ++ (t, wait_handler t u n ++ rest) :: P2)
+  (Hlen1 : length vs1 = n) (Hlen2 : length vs2 = n) (Hn : n <> 0),
+  exec_star (Some P) G
+    (events_max_vc (C + u) (C + t) t n ++ events_inc_vc (C + u) t)
+    (mops_max_vc (C + u) (C + t) vs1 vs2 t n ++ mops_inc_vc' (C + u) v t u)
+    (Some (P1 ++ (t, rest) :: P2))
+    (upd_env (upd_env G t tmp2 (Peano.max (last vs1 0) (last vs2 0)))
+             t tmp1 (v + 1)).
+Proof.
+  intros; eapply exec_t_exec, wait_handler_spec_t; auto.
 Qed.
 
 (* Note that for now, we assign metadata to a block, rather than to
@@ -1118,7 +926,6 @@ let instrument := fix f p t :=
  | Unlock l   => unlock_handler t l zt  tmp1++ [ins]
  | Spawn u li =>  spawn_handler t u zt ++ [Spawn u (instrument li u)] 
  | Wait u     => [ins] ++ wait_handler t u zt
- (* the wait_handler should be called after the wait returns*)
  | _          => [ins]
 end).
 
@@ -1221,7 +1028,8 @@ Proof.
   induction li; clarify.
 Qed.
 
-(* an instruction is safe iff it only access the part of memory that does not hold meta locations*)
+(* an instruction is safe if it only accesses the part of memory that does not
+   hold meta locations. *)
 Fixpoint safe_instr (i : instr) :=
   let list_safe := fix list_safe l :=
     match l with
@@ -1236,7 +1044,7 @@ Fixpoint safe_instr (i : instr) :=
   | Unlock m => ~meta_loc (m, 0) /\ m < zl
   | Spawn u li => u < zt /\ list_safe li
   | Wait u => u < zt
-  | _ => True
+  | Assert_le _ _ => True (* should this be False? *)
   end.
 
 (* all the instructions in P are safe*)
@@ -1277,12 +1085,19 @@ Proof.
   specialize (Hle a); rewrite <- leb_le in Hle; clarify.
 Qed.
 
-(* updates to different stacks(per-thread) don't interfere with each other*)
-Lemma upd_old_t : forall G t1 a1 v1 t2 a2 (Ht : t1 <> t2),
-  upd_env G t1 a1 v1 t2 a2 = G t2 a2.
-Proof.
-  intros; unfold upd_env, upd; clarify.
-Qed.
+Lemma C_meta : forall t (Ht : t < zt) o, meta_loc (C + t, o).
+Proof. intros; unfold meta_loc; simpl; omega. Qed. 
+
+Lemma X_meta : forall v (Ht : v < zv) o, meta_loc (X + v, o).
+Proof. intros; unfold meta_loc; simpl; omega. Qed.
+Lemma R_meta : forall v (Ht : v < zv) o, meta_loc (R + v, o).
+Proof. intros; unfold meta_loc; simpl; omega. Qed.
+
+Lemma W_meta : forall v (Ht : v < zv) o, meta_loc (W + v, o).
+Proof. intros; unfold meta_loc; simpl; omega. Qed.
+
+Lemma L_meta : forall l (Ht : l < zl) o, meta_loc (L + l, o).
+Proof. intros; unfold meta_loc; simpl; omega. Qed.
 
 (* all the memory operations only access meta locations*)
 Lemma mops_hb_check_meta : forall l1 l2 n x t c (Hx : x < zv) (Ht : t < zt)
@@ -1291,18 +1106,8 @@ Proof.
   induction l1; clarify.
   destruct n; clarify.
   destruct l2; clarify.
-  destruct Hin as [? | [? | ?]].
-  destruct H; clarify.
-  - unfold meta_loc; clarify; omega.
-  - destruct H; clarify.
-    +unfold meta_loc; clarify; omega.
-    +eapply IHl1; eauto.
-  
-- clarify.
-  unfold meta_loc; clarify; omega.
-- destruct H; clarify.
-  + unfold meta_loc; clarify; omega.
-  + eapply IHl1; eauto.
+  destruct Hin as [[? | [? | ?]] | [? | [? | ?]]]; clarify;
+    try apply W_meta; try apply R_meta; try apply C_meta; eauto.
 Qed.
 
 (* all the memory operations only access meta locations*)
@@ -1312,10 +1117,8 @@ Proof.
   induction l1; clarify.
   destruct n; clarify.
   destruct l2; clarify.
-  destruct Hin;
-  destruct n; clarify; destruct l2; clarify;
-  repeat (destruct H; clarify;  [unfold meta_loc; clarify; omega |]);
-  eauto.
+  destruct Hin as [[? | [? | [? | ?]]] | [? | [? | [? | ?]]]]; clarify;
+    try apply L_meta; try apply C_meta; eauto.
 Qed.
 
 Notation lower := (@lower _ _ _ _ _ Base).
@@ -1494,7 +1297,7 @@ Proof.
    +destruct (eq_dec v tmp2). clarify. eauto.
   -destruct (eq_dec tmp1 v). clarify. eauto.
   -destruct (eq_dec tmp2 v). clarify. eauto. 
-Qed.    
+Qed.
  
 Lemma eval_old: forall G1 G2 t0 v1 v2 e (HGsim: env_sim G1 G2) (Htmp1: expr_fresh tmp1 e) (Htmp2: expr_fresh tmp2 e), eval (upd_env (upd_env G2 t0 tmp1 v1) t0 tmp2 v2 t0) e = eval (G1 t0) e.
 Proof.
@@ -1556,16 +1359,13 @@ Proof.
   inversion H; intro; clarify.
 Qed.
 
-Lemma mops_set_vc_meta_cl: forall vs n u t c (Hx : u < zl) (Ht : t < zt)
+Lemma mops_set_vc_meta_cl: forall n vs u t c (Hx : u < zl) (Ht : t < zt)
   (Hin : In c (mops_set_vc (C + t) (L + u) n t vs )), meta_loc (loc_of c).
 Proof.
-  induction vs; clarify.
   induction n; clarify.
-  destruct n; clarify.
-  destruct Hin; clarify; [ unfold meta_loc; clarify; omega | ].
-  destruct H; clarify. unfold meta_loc; simpl; omega. 
-  
-  specialize(IHvs n u t c Hx Ht H). auto.
+  destruct vs; clarify.
+  destruct Hin as [? | [? | ?]]; clarify; try apply C_meta; try apply L_meta;
+    eauto.
 Qed.
 
 
@@ -1673,9 +1473,8 @@ Proof.
   induction l1; clarify.
   destruct n; clarify.
   destruct l2; clarify.
-  specialize (IHl1 l2 n u t c); clarify.
-  repeat (destruct Hin as [Hin | Hin]); clarify; unfold meta_loc; simpl;
-    abstract omega.
+  destruct Hin as [[? | [? | [? | ?]]] | [? | [? | [? | ?]]]]; clarify;
+    try apply C_meta; eauto.
 Qed.
 
 Lemma hb_check_prog : forall C1 C2 z t vs1 vs2,
@@ -1763,7 +1562,9 @@ Inductive iexec P G t :
       (Hpass : eval (G t) e1 <= eval (G t) e2) :
       iexec P G t [] [] (P1 ++ (t, rest) :: P2) G.
 
-Lemma env_sim_refl : forall G, env_sim G G.
+Require Import RelationClasses.
+
+Instance env_sim_refl : Reflexive env_sim.
 Proof. repeat intro; auto. Qed.
 
 Corollary eval_old' : forall G t v1 v2 e
@@ -1774,29 +1575,43 @@ Proof.
   apply env_sim_refl.
 Qed.
 
-Lemma iexec_exec : forall P G t lo lc P' G' (Hiexec : iexec P G t lo lc P' G'),
-  exec_star (Some P) G lo lc (Some P') G'.
+Lemma last_f : forall A B (f : A -> A -> B) d d' l1 l2
+  (Hl1 : l1 <> []) (Hl2 : l2 <> []) (Hlen : length l1 = length l2),
+  last (map (fun x => f (fst x) (snd x)) (combine l1 l2)) d =
+  f (last l1 d') (last l2 d').
 Proof.
-  intros; induction Hiexec; clarify.
-  - eapply exec_step'.
+  induction l1; clarify.
+  destruct l2; clarify.
+  destruct (nil_dec l1).
+  - destruct l2; clarify.
+  - destruct (nil_dec l2); [destruct l1; clarify|].
+    rewrite last_cons, last_cons, last_cons; auto.
+    destruct (combine l1 l2) eqn: Hcom; clarify.
+    destruct l1, l2; clarify.
+Qed.
+
+Lemma iexec_exec_t : forall P G t lo lc P' G'
+  (Hiexec : iexec P G t lo lc P' G'),
+  exec_star_t t (Some P) G lo lc (Some P') G'.
+Proof.
+  intros; inversion Hiexec; clarify.
+  - eapply exec_step_t'.
     + apply exec_assign; eauto.
-    + apply exec_refl.
+    + apply exec_refl_t.
     + auto.
     + auto.
-  - eapply exec_step_inv.
-    eapply exec_step_inv.
-    + apply load_handler_norace_spec; try (apply Hle); eauto.
+  - eapply exec_step_inv_t'.
+    eapply exec_step_inv_t'; auto.
+    + apply load_handler_norace_spec_t; try (apply Hle); eauto.
       unfold load_handler.
       simpl; do 2 rewrite <- (app_assoc (hb_check _ _ _ _ _)); eauto.
     + apply exec_load; eauto.
-    + eauto.
-    + eauto.
     + apply exec_unlock; eauto.
-    + clarsimp.
-    + clarsimp.
-  - eapply exec_step_inv.
-    eapply exec_step_inv.
-    + apply store_handler_norace_spec.
+    + simpl; repeat rewrite <- app_assoc; auto.
+    + simpl; repeat rewrite <- app_assoc; auto.
+  - eapply exec_step_inv_t'.
+    eapply exec_step_inv_t'; auto.
+    + apply store_handler_norace_spec_t.
       * unfold store_handler.
         simpl; eauto.
       * apply Hlen1.
@@ -1805,66 +1620,54 @@ Proof.
       * auto.
       * auto.
     + apply exec_store; eauto.
-    + eauto.
-    + eauto.
     + apply exec_unlock; eauto.
-    + clarsimp.
-    + clarsimp.
+    + simpl; repeat rewrite <- app_assoc; auto.
+    + simpl; repeat rewrite <- app_assoc; auto.
       rewrite eval_old'; auto.
-  - eapply exec_step'.
+  - eapply exec_step_t'.
     + eapply exec_lock; eauto.
-    + apply lock_handler_spec; eauto.
+    + apply lock_handler_spec_t; eauto.
+      apply zt_non_zero.
     + auto.
     + auto.
-  - generalize zt_non_zero; destruct zt; clarify.
-    destruct (length vs) eqn: Hlen1; [clarify|].
-    inversion Hlen; clarify.
-    destruct (nil_dec vs); [clarify|].
-    eapply exec_step_inv.
-    + eapply unlock_handler_spec_n with (v := last vs 0).
-      { eauto. }
-      { rewrite (app_removelast_last 0 n0), app_length, Nat.add_1_r in Hlen1;
-          inversion Hlen1; eauto. }
+  - eapply exec_step_inv_t'.
+    + apply unlock_handler_spec_t; eauto.
     + apply exec_unlock; eauto.
-    + clarsimp.
-    + rewrite <- app_removelast_last; clarsimp.
-
-  - generalize zt_non_zero; destruct zt; clarify.
-    destruct (nil_dec vs1); [clarify|].
-    destruct (nil_dec vs2); [clarify|].
-    eapply exec_step_inv.
-    + eapply spawn_handler_spec_n.
-      { simpl; eauto. }
-      { rewrite (app_removelast_last 0 n0), app_length, Nat.add_1_r in Hlen1;
-          inversion Hlen1; eauto. }
-      { rewrite (app_removelast_last 0 n1), app_length, Nat.add_1_r in Hlen2;
-          inversion Hlen2; eauto. }
-      { auto. }
-    + apply exec_spawn; eauto.
-      intro Hin. contradiction Hnew.
-      rewrite map_app in *. simpl in *. auto.
-    + clarsimp.
-    + repeat rewrite <- app_removelast_last; clarsimp.
-    
-  - generalize zt_non_zero; destruct zt; clarify.
-    destruct (nil_dec vs1); [clarify|].
-    destruct (nil_dec vs2); [clarify|].
-    eapply exec_step'.
-    + apply exec_wait; auto.
-    +
-      apply wait_handler_spec_n.
-      { simpl; eauto. }
-      { rewrite (app_removelast_last 0 n0), app_length, Nat.add_1_r in Hlen1;
-          inversion Hlen1; simpl; eauto. }
-      { rewrite (app_removelast_last 0 n1), app_length, Nat.add_1_r in Hlen2;
-          inversion Hlen2; eauto. }
-    + clarsimp. 
-    + repeat rewrite <- app_removelast_last; clarsimp.
-  - eapply exec_step'.
+    + rewrite <- app_assoc; auto.
+    + rewrite <- app_assoc; auto.
+  - eapply exec_step_inv_t'.
+    + apply spawn_handler_spec_t.
+      * eauto.
+      * apply Hlen1.
+      * apply Hlen2.
+      * auto.
+    + generalize zt_non_zero; intro.
+      erewrite last_f.
+      * apply exec_spawn; auto.
+        intro; contradiction Hnew.
+        rewrite map_app, in_app in *; clarify.
+      * intro; clarify.
+      * intro; clarify.
+      * rewrite Hlen1; auto.
+    + rewrite <- app_assoc; auto.
+    + rewrite <- app_assoc; auto.
+  - eapply exec_step_t'.
+    + apply exec_wait; eauto.
+    + apply wait_handler_spec_t; eauto.
+      apply zt_non_zero.
+    + auto.
+    + auto.
+  - eapply exec_step_t'.
     + eapply exec_assert_pass; eauto.
-    + apply exec_refl.
+    + apply exec_refl_t.
     + auto.
     + auto.
+Qed.
+
+Corollary iexec_exec : forall P G t lo lc P' G'
+  (Hiexec : iexec P G t lo lc P' G'), exec_star (Some P) G lo lc (Some P') G'.
+Proof.
+  intros; eapply exec_t_exec, iexec_exec_t; eauto.
 Qed.
 
 Inductive iexec_star : state -> env ->
